add inductive parse error type

coq/Parser.v
@@ -11,24 +11,29 @@ Record frame := Fr { loc : location
                    ; sem : forest
                    }.                               
 
-Definition p_stack := (frame * list frame)%type.
+Definition parser_stack := (frame * list frame)%type.
 
-Definition locStackOf (stk : p_stack) : location_stack :=
+Definition locStackOf (stk : parser_stack) : location_stack :=
   let (fr, frs) := stk in (fr.(loc), map loc frs).
   
 Record parser_state    := Pst { avail  : NtSet.t
-                              ; stack  : p_stack               
+                              ; stack  : parser_stack     
                               ; tokens : list token
                               }.
+
+Inductive error_type :=
+| InvalidState    : error_type
+| PredictionError : string -> error_type
+| LeftRecursion   : nonterminal -> error_type.
 
 Inductive step_result := StepAccept : forest -> step_result
                        | StepReject : string -> step_result
                        | StepK      : parser_state -> step_result
-                       | StepError  : string -> step_result.
+                       | StepError  : error_type -> step_result.
 
 Inductive parse_result := Accept : forest -> parse_result
                         | Reject : string -> parse_result
-                        | Error  : string -> parse_result.
+                        | Error  : error_type -> parse_result.
 
 Definition step (g : grammar) (st : parser_state) : step_result :=
   match st with
@@ -47,8 +52,8 @@ Definition step (g : grammar) (st : parser_state) : step_result :=
         (* nonempty stack --> return to caller frame *)
         | (Fr (Loc xo_cr pre_cr suf_cr) sv_cr) :: frs_tl =>
           match suf_cr with
-          | []                 => StepError "impossible"
-          | T _ :: _           => StepError "impossible"
+          | []                 => StepError InvalidState
+          | T _ :: _           => StepError InvalidState
           | NT x :: suf_cr_tl => 
             let cr' := Fr (Loc xo_cr (pre_cr ++ [NT x]) suf_cr_tl)
                           (sv_cr ++ [Node x sv])
@@ -78,42 +83,13 @@ Definition step (g : grammar) (st : parser_state) : step_result :=
             let callee := Fr (Loc (Some x) [] rhs) []
             in  StepK (Pst (NtSet.remove x av) (callee, fr :: frs) ts)
           | PredReject    => StepReject "prediction found no viable right-hand sides"
-          | PredError msg => StepError msg
+          | PredError msg => StepError (PredictionError msg)
           end
         else
-          StepError "left recursion detected"
+          StepError (LeftRecursion x)
       end
     end
   end.
-
-(*Definition headFrameSize (fr : parser_frame) : nat :=
-  List.length fr.(syms).
-
-Definition headFrameScore (fr : parser_frame) (b : nat) (e : nat) : nat :=
-  headFrameSize fr * (b ^ e).
-
-Definition tailFrameSize (fr : parser_frame) : nat :=
-  match fr.(syms) with
-  | [] => 0
-  | _ :: syms' => List.length syms'
-  end.
-
-Definition tailFrameScore (fr : parser_frame) (b : nat) (e : nat) : nat :=
-  tailFrameSize fr * (b ^ e).
-
-Fixpoint tailFramesScore (frs : list parser_frame) (b : nat) (e : nat) : nat :=
-  match frs with
-  | [] => 0
-  | fr :: frs' => tailFrameScore fr b e + tailFramesScore frs' b (1 + e)
-  end.
-
-Definition stackScore (stk : parser_stack) (b : nat) (e : nat) : nat :=
-  let (hf, tfs) := stk
-  in  headFrameScore hf b e + tailFramesScore tfs b (1 + e).
-
-Definition stackHeight (stk : parser_stack) : nat :=
-  let (_, frs) := stk in List.length frs.
- *)
 
 Definition meas (g : grammar) (st : parser_state) : nat * nat * nat :=
   match st with
@@ -122,228 +98,6 @@ Definition meas (g : grammar) (st : parser_state) : nat * nat * nat :=
     let e := NtSet.cardinal av in
     (List.length ts, stackScore (locStackOf stk) (1 + m) e, stackHeight stk)
   end.
-
-(*
-Lemma meas_unfold : 
-  forall st tbl, meas st tbl = (List.length st.(tokens), 
-                                stackScore st.(stack) (1 + maxEntryLength tbl) (NtSet.cardinal st.(avail)),
-                                stackHeight st.(stack)).
-Proof. 
-  auto.
-Qed.
- *)
-
-(*
-Definition nat_triple_lex : relation (nat * nat * nat) :=
-  triple_lex nat nat nat lt lt lt.
-
-Lemma headFrameScore_nil :
-  forall fr b e,
-    fr.(syms) = [] -> headFrameScore fr b e = 0.
-Proof.
-  intros fr b e Hfr.
-  unfold headFrameScore. unfold headFrameSize.
-rewrite Hfr; auto.
-Qed.
-
-Lemma tailFrameScore_cons :
-  forall fr sym gamma b e,
-    fr.(syms) = sym :: gamma -> tailFrameScore fr b e = List.length gamma * (b ^ e).
-Proof.
-  intros fr sym gamma b e Hfr.
-  unfold tailFrameScore. unfold tailFrameSize.
-  rewrite Hfr; auto.
-Qed.
-
-Lemma stackScore_head_frame_nil :
-  forall fr frs b e, 
-    fr.(syms) = [] 
-    -> stackScore (fr, frs) b e = tailFramesScore frs b (1 + e).
-Proof.
-  intros fr frs b e Hfr.  
-  unfold stackScore. unfold headFrameScore. unfold headFrameSize.
-  rewrite Hfr; simpl; auto.
-Qed.
-
-Lemma stackScore_pre_return :
-  forall fr fr' sym gamma frs b e, 
-    fr.(syms) = nil
-    -> fr'.(syms) = sym :: gamma
-    -> stackScore (fr, fr' :: frs) b e = 
-       (List.length gamma * b ^ (1 + e)) + tailFramesScore frs b (2 + e).
-Proof.
-  intros fr fr' sym gamma frs b e Hfr Hfr'.
-  rewrite stackScore_head_frame_nil; auto.
-  simpl.
-  erewrite tailFrameScore_cons; eauto.
-Qed.
-
-Lemma post_return_state_lt_pre_return_state :
-  forall st st' ts callee caller caller' frs x gamma av tbl,
-    st = parserState av (callee, caller :: frs) ts
-    -> st' = parserState (NtSet.add x av) (caller', frs) ts
-    -> callee.(syms) = []
-    -> caller.(syms) = NT x :: gamma
-    -> caller'.(syms) = gamma
-    -> nat_triple_lex (meas st' tbl) (meas st tbl).
-Proof.
-  intros st st' ts callee caller caller' frs x gamma av tbl Hst Hst' Hnil Hcons Htl; subst.
-  unfold meas; simpl.
-  rewrite headFrameScore_nil with (fr := callee); simpl; auto.
-  erewrite tailFrameScore_cons; eauto.
-  unfold headFrameScore. unfold headFrameSize.
-  destruct (NtSet.mem x av) eqn:Hm.
-  - (* x is already in av, so the cardinality stays the same *)
-    rewrite add_cardinal_1; auto.
-    pose proof nonzero_exponents_lt_stackScore_le as Hle. 
-    specialize (Hle (List.length caller'.(syms))
-                  (S (maxEntryLength tbl)) 
-                  (NtSet.cardinal av)
-                  (S (NtSet.cardinal av))
-                  (S (NtSet.cardinal av))
-                  (S (S (NtSet.cardinal av)))
-                  frs).
-    apply le_lt_or_eq in Hle.
-    + destruct Hle as [Hlt | Heq]; subst.
-      * apply triple_snd_lt; auto.
-      * rewrite Heq.
-        apply triple_thd_lt; auto.
-    + split; auto.
-      eapply mem_true_cardinality_gt_0; eauto.
-    + split; auto.
-      omega.
-  - (* x isn't in av, so the cardinality increase by 1 *)
-    rewrite add_cardinal_2; auto.
-    apply triple_thd_lt; auto.
-Qed.
-
-Lemma gamma_in_table_length_in_entryLengths :
-  forall k gamma tbl,
-    In (k, gamma) (ParseTable.elements tbl)
-    -> In (List.length gamma) (entryLengths tbl).
-Proof.
-  intros k gamma tbl Hin.
-  unfold entryLengths.
-  induction (ParseTable.elements tbl) as [| (k', gamma') prs IH]; inv Hin; simpl in *.
-  - inv H; auto.
-  - apply IH in H; auto.
-Qed.
-
-Module Export PF := WFacts ParseTable.
-
-Lemma pt_findA_In :
-  forall (k : ParseTable.key) (gamma : list symbol) (l : list (ParseTable.key * list symbol)),
-    findA (PF.eqb k) l = Some gamma
-    -> In (k, gamma) l.
-Proof.
-  intros.
-  induction l.
-  - inv H.
-  - simpl in *.
-    destruct a as (k', gamma').
-    destruct (PF.eqb k k') eqn:Heq.
-    + inv H.
-      unfold PF.eqb in *.
-      destruct (PF.eq_dec k k').
-      * subst; auto.
-      * inv Heq.
-    + right; auto.
-Qed.
-
-Lemma find_Some_gamma_in_table :
-  forall k (gamma : list symbol) tbl,
-    ParseTable.find k tbl = Some gamma -> In (k, gamma) (ParseTable.elements tbl).
-  intros k gamma tbl Hf.
-  rewrite elements_o in Hf.
-  apply pt_findA_In in Hf; auto.
-Qed.
-
-Lemma tbl_lookup_result_le_max :
-  forall k tbl gamma,
-    ParseTable.find k tbl = Some gamma
-    -> List.length gamma <= maxEntryLength tbl.
-Proof.
-  intros k tbl gamma Hf.
-  unfold maxEntryLength.
-  apply list_element_le_listMax.
-  apply gamma_in_table_length_in_entryLengths with (k := k).
-  apply find_Some_gamma_in_table; auto.
-Qed.  
-
-Lemma tbl_lookup_result_lt_max_plus_1 :
-  forall k tbl gamma,
-    ParseTable.find k tbl = Some gamma
-    -> List.length gamma < 1 + maxEntryLength tbl.
-Proof.
-  intros k tbl gamma Hf.
-  apply (tbl_lookup_result_le_max k tbl gamma) in Hf; omega.
-Qed.
-
-Lemma post_push_state_lt_pre_push_st :
-  forall st st' ts callee caller frs x gamma_caller gamma_callee av tbl,
-    st = parserState av (caller, frs) ts
-    -> st' = parserState (NtSet.remove x av) (callee, caller :: frs) ts
-    -> caller.(syms) = NT x :: gamma_caller
-    -> callee.(syms)  = gamma_callee
-    -> ParseTable.find (x, peek ts) tbl = Some gamma_callee
-    -> NtSet.mem x av = true
-    -> nat_triple_lex (meas st' tbl) (meas st tbl).
-Proof.
-  intros st st' ts callee caller frs x gamma_caller gamma_callee av tbl Hst Hst' Hcaller Hcallee Hfind Hmem; subst.
-  apply triple_snd_lt; simpl.
-  rewrite remove_cardinal_1; auto.
-  unfold headFrameScore. unfold headFrameSize.
-  unfold tailFrameScore. unfold tailFrameSize. rewrite Hcaller.
-  simpl.
-rewrite plus_assoc. 
-apply plus_lt_compat_r.
-apply plus_lt_compat_r.
-assert (remove_cardinal_minus_1 : forall x s,
-           NtSet.mem x s = true
-           -> NtSet.cardinal (NtSet.remove x s) = 
-              NtSet.cardinal s - 1).
-       
-{ intros x' s Hm.
-  replace (NtSet.cardinal s) with (S (NtSet.cardinal (NtSet.remove x' s))).
-  - omega.
-  - apply remove_cardinal_1; auto. }
-rewrite remove_cardinal_minus_1; auto.
-apply less_significant_value_lt_more_significant_digit.
-  - eapply tbl_lookup_result_lt_max_plus_1; eauto.
-  - erewrite <- remove_cardinal_1; eauto. 
-    omega.
-Qed.
-
-Lemma step_meas_lt :
-  forall tbl st st',
-    step tbl st = StepK st'
-    -> nat_triple_lex (meas st' tbl) (meas st tbl).
-Proof.
-  intros tbl st st' Hs.
-  unfold step in Hs.
-  destruct st as [av [fr frs] ts].
-  destruct fr as [gamma sv].
-  destruct gamma as [| [y | x] gamma'].
-  - (* return from the current frame *)
-    destruct frs as [| caller frs']; try congruence.
-    destruct caller as [gamma_caller sv_caller]. 
-    destruct gamma_caller as [| [y | x] gamma_caller']; try congruence.
-    inv Hs.
-    eapply post_return_state_lt_pre_return_state; simpl; eauto.
-    simpl; auto.
-  - (* terminal case *) 
-    destruct ts as [| (y', l) ts']; try congruence.
-    destruct (t_eq_dec y' y); try congruence.
-    inv Hs.
-    apply triple_fst_lt; simpl; auto.
-  - (* nonterminal case -- push a new frame onto the stack *)
-    destruct (NtSet.mem x av) eqn:Hm; try congruence.
-    destruct (ParseTable.find (x, peek ts) tbl) as [gamma |] eqn:Hf; try congruence.
-    inv Hs.
-    eapply post_push_state_lt_pre_push_st; eauto.
-    simpl; eauto.
-Qed.
- *)
 
 Lemma state_lt_after_return :
   forall g st st' ts callee caller caller' frs x x' suf_cr_tl av,
@@ -452,7 +206,7 @@ Fixpoint multistep (g  : grammar)
   match step g st as res return step g st = res -> _ with
   | StepAccept sv    => fun _  => Accept sv
   | StepReject s     => fun _  => Reject s
-  | StepError s      => fun _  => Error s
+  | StepError e      => fun _  => Error e
   | StepK st'        => fun Hs => multistep g st' (StepK_st_acc _ _ _ a Hs)
   end eq_refl.
 
